Evaluation of bterms

BTerm.thy
@@ -1,46 +1,287 @@
-theory BTerm imports Locales
+theory BTerm imports Valuation
 begin
 
 section \<open>De Bruijn Term\<close>
 
-subsection \<open>Terms\<close>
+subsection \<open>De Bruijn Terms\<close>
 
 datatype bterm = 
   FreeVar variable \<open>bterm list\<close>
 | BoundVar nat
 | Abstr abstraction \<open>bterm list\<close>
 
-subsection \<open>Free Atoms\<close>
-
-datatype atom =
-  Var variable nat
-| Unbound nat 
-
-type_synonym atoms = "atom set"
+subsection \<open>Unbound and Free Variables\<close>
 
 context sigloc begin
 
-fun freeAtomsAt :: "nat \<Rightarrow> bterm \<Rightarrow> atoms" where 
-  "freeAtomsAt level (FreeVar x ts) = 
-     (\<section>fold atoms = {Var x (length ts)}, t=ts!_. atoms \<union> freeAtomsAt level t)"
-| "freeAtomsAt level (BoundVar i) = 
-     (if i < level then {} else {Unbound (i - level)})"
-| "freeAtomsAt level (Abstr a ts) = 
-     (\<section>fold atoms = {}, t=ts!_. atoms \<union> freeAtomsAt (level + \<section>v a) t)" 
+definition raise_indices :: "nat set \<Rightarrow> nat \<Rightarrow> nat set" (infixl ".\<up>" 80)
+  where "raise_indices I m = { i + m | i. i \<in> I }"
 
-definition freeAtoms :: "bterm \<Rightarrow> atoms" where
-  "freeAtoms t = freeAtomsAt 0 t"
+definition lower_indices :: "nat set \<Rightarrow> nat \<Rightarrow> nat set" (infixl ".\<down>" 80)
+  where "I .\<down> m = { i - m | i. i \<in> I \<and> i \<ge> m }"
 
-definition unboundAtoms :: "nat set \<Rightarrow> atoms" ("\<up>") where
-  "\<up>ubs = { Unbound u | u. u \<in> ubs }"
+lemma raise_indices_0[simp]: "I .\<up> 0 = I"
+  by (simp add: raise_indices_def)
+
+lemma lower_indices_0[simp]: "I .\<down> 0 = I"
+  by (simp add: lower_indices_def)
+
+lemma raise_indices_mono: "A \<subseteq> B \<Longrightarrow> A .\<up> m \<subseteq> B .\<up> m"
+  using raise_indices_def by auto
+
+lemma lower_indices_mono: "A \<subseteq> B \<Longrightarrow> A .\<down> m \<subseteq> B .\<down> m"
+  using lower_indices_def by auto
+
+lemma raise_lower_indices_le[simp]: "n \<le> m \<Longrightarrow> I .\<up> m .\<down> n = I .\<up> (m - n)"
+  by (auto simp add: lower_indices_def raise_indices_def)
+
+lemma raise_lower_indices_ge[simp]: "n \<ge> m \<Longrightarrow> I .\<up> m .\<down> n = I .\<down> (n - m)"
+  by (auto simp add: lower_indices_def raise_indices_def)
+
+lemma erase_bottom_indices: "i \<in> I .\<down> m .\<up> m \<Longrightarrow> i \<ge> m \<and> i \<in> I"
+  using lower_indices_def raise_indices_def by force
+
+lemma undo_raise_indices: "i \<in> I .\<up> m \<Longrightarrow> i - m \<in> I"
+  using raise_indices_def by fastforce
+
+fun unbounds :: "bterm \<Rightarrow> nat set"  where 
+  "unbounds (FreeVar x ts) = (\<section>fold I = {}, t=ts!_. I \<union> unbounds t)"
+| "unbounds (BoundVar i) = {i}"
+| "unbounds (Abstr a ts) = (\<section>fold I = {}, t=ts!_. I \<union> unbounds t) .\<down> \<section>v a" 
+
+lemma unbounds_freeVar_arg: "\<And> i. i < length ts \<Longrightarrow> unbounds (ts ! i) \<subseteq> unbounds (FreeVar x ts)"
+  by (auto simp add:  union_indexed_fold)
+
+lemma unbounds_abstr: 
+  assumes i: "k < length ts"
+  shows "unbounds (ts ! k) \<subseteq> unbounds (Abstr a ts) .\<up> \<section>v a \<union> nats (\<section>v a)"
+proof - 
+  {
+    fix i :: nat
+    assume i: "i \<in> unbounds (ts ! k) \<and> i \<ge> \<section>v a"
+    have "i - \<section>v a \<in> unbounds (Abstr a ts)"
+      apply (auto simp add: union_indexed_fold)
+      using assms(1) i lower_indices_def by auto
+    have "i \<in> unbounds (Abstr a ts) .\<up> \<section>v a"
+      apply (auto simp add: union_indexed_fold)
+      by (smt (verit, ccfv_SIG) CollectI UnionI assms(1) i le_add_diff_inverse2 lower_indices_def 
+          raise_indices_def)
+  }
+  then show ?thesis by force
+qed
+
+fun bfrees :: "bterm \<Rightarrow> variables" where 
+  "bfrees (FreeVar x ts) = 
+     (\<section>fold X = {(x, length ts)}, t=ts!_. X \<union> bfrees t)"
+| "bfrees (BoundVar i) = {}" 
+| "bfrees (Abstr a ts) = (\<section>fold X = {}, t=ts!_. X \<union> bfrees t)" 
+
+lemma bfrees_freeVar_arg: "\<And> i. i < length ts \<Longrightarrow> bfrees (ts ! i) \<subseteq> bfrees (FreeVar x ts)"
+  by (auto simp add: union_indexed_fold)
+
+lemma bfrees_abstr_arg: "\<And> i. i < length ts \<Longrightarrow> bfrees (ts ! i) \<subseteq> bfrees (Abstr a ts)"
+  by (auto simp add: union_indexed_fold)
 
 subsection \<open>Wellformedness\<close>
 
-fun bt_wf :: "bterm \<Rightarrow> bool" where
-  "bt_wf (FreeVar x ts) = (\<forall> t=ts!_. bt_wf t)"
-| "bt_wf (BoundVar i) = True"
-| "bt_wf (Abstr a ts) = (\<checkmark>a \<and> \<section>a a = length ts \<and> 
-     (\<forall> t=ts!i. bt_wf t \<and> freeAtoms t \<inter> \<up>(nats (\<section>v a)) \<subseteq> \<up>(a!\<natural>i)))"
+fun bwf :: "bterm \<Rightarrow> bool" where
+  "bwf (FreeVar x ts) = (\<forall> t=ts!_. bwf t)"
+| "bwf (BoundVar i) = True"
+| "bwf (Abstr a ts) = (\<checkmark>a \<and> \<section>a a = length ts \<and> 
+     (\<forall> t=ts!i. bwf t \<and> unbounds t \<inter> nats (\<section>v a) \<subseteq> a!\<natural>i))"
+
+lemma bwf_freeVar_arg: "bwf (FreeVar x ts) \<Longrightarrow> i < length ts \<Longrightarrow> bwf (ts!i)"
+  by auto
+
+lemma bwf_abstr_arg: "bwf (Abstr a ts) \<Longrightarrow> i < length ts \<Longrightarrow> bwf (ts!i)"
+  by (simp add: list_indexed_forall_def)
+
+lemma unbounds_bwf_abstr: 
+  assumes i: "k < length ts"
+  assumes wf: "bwf (Abstr a ts)"
+  shows "unbounds (ts ! k) \<subseteq> unbounds (Abstr a ts) .\<up> \<section>v a \<union> a!\<natural>k"
+proof - 
+  {
+    fix i :: nat
+    assume i: "i \<in> unbounds (ts ! k) \<and> i \<ge> \<section>v a"
+    have "i - \<section>v a \<in> unbounds (Abstr a ts)"
+      apply (auto simp add: union_indexed_fold)
+      using assms(1) i lower_indices_def by auto
+    have "i \<in> unbounds (Abstr a ts) .\<up> \<section>v a"
+      apply (auto simp add: union_indexed_fold)
+      by (smt (verit, ccfv_SIG) CollectI UnionI assms(1) i le_add_diff_inverse2 lower_indices_def 
+          raise_indices_def)
+  }
+  note left = this
+  {
+    fix i :: nat
+    assume i: "i \<in> unbounds (ts ! k) \<and> i < \<section>v a"
+    have "unbounds (ts!k) \<inter> nats (\<section>v a) \<subseteq> a!\<natural>k" using wf
+      by (simp add: assms(1) list_indexed_forall_def)
+    with i have i': "i \<in> a!\<natural>k" by (simp add: in_mono)
+  }
+  note right = this
+  show ?thesis using left right by fastforce
+qed
+
+lemma upper_bound_unbounds_abstr_arg:
+  assumes i:"i \<in> \<Union> { unbounds t | t. t \<in> set ts }" 
+  shows "i \<in> unbounds (Abstr a ts) .\<up> \<section>v a \<union> (nats (\<section>v a))"
+proof -
+  have conv: "\<Union> { unbounds t | t. t \<in> set ts } =  \<Union> { unbounds (ts!k) | k. k < length ts }"
+    by (metis in_set_conv_nth)
+  with i have "i \<in> \<Union> { unbounds (ts!k) | k. k < length ts }"
+    by auto
+  then have "i \<in> \<Union> { unbounds (Abstr a ts).\<up> \<section>v a \<union> (nats (\<section>v a)) | k. k < length ts }"
+    using unbounds_abstr by fastforce
+  then show ?thesis by blast
+qed
+
+lemma upper_bound_erased_unbounds_abstr_arg:
+  assumes i:"i \<in> \<Union> { unbounds t | t. t \<in> set ts } .\<down> \<section>v a .\<up> \<section>v a" 
+  shows "i \<in> unbounds (Abstr a ts) .\<up> \<section>v a"
+proof - 
+  have i1: "i \<in> unbounds (Abstr a ts) .\<up> \<section>v a \<union> (nats (\<section>v a))"
+    by (meson erase_bottom_indices i upper_bound_unbounds_abstr_arg)
+  have i2: "i \<ge> \<section>v a"
+    using erase_bottom_indices i by blast
+  from i1 i2 show ?thesis by fastforce
+qed
+
+end
+
+subsection \<open>Environments\<close>
+
+type_synonym 'a env = "nat \<Rightarrow> 'a"
+
+definition update_env :: "'a env \<Rightarrow> nat \<Rightarrow> nat set \<Rightarrow> 'a list \<Rightarrow> 'a env" 
+  ("_\<up>_{_ := _}" [1000, 51, 51, 51] 1000)
+where 
+  "update_env env m js xs = (\<lambda> j. 
+     (case index_of j (sorted_list js) of
+        Some i \<Rightarrow> xs!i
+      | None \<Rightarrow> env (j - m)))"
+
+abbreviation raise_env :: "'a env \<Rightarrow> nat \<Rightarrow> 'a env"
+  ("_\<up>_{}" [1000, 51] 1000)
+where 
+  "env \<up> m {} \<equiv> env \<up> m { {} := [] }"
+
+lemma env_app_noupdate: "finite js \<Longrightarrow> j \<notin> js \<Longrightarrow> env \<up> m { js := xs } j = env \<up> m {} j"
+  by (simp add: update_env_def no_index_sorted_list)
+
+lemma env_raised_app: "env \<up> m {} j = env (j - m)"
+  by (simp add: no_index_sorted_list update_env_def)
+
+lemma env_app_update: 
+  "finite js \<Longrightarrow> j \<in> js \<Longrightarrow> env \<up> m { js := us } j = us ! the (index_of j (sorted_list js))"
+  by (metis index_of_is_None option.case_eq_if set_sorted_list update_env_def)
+  
+context algloc begin
+
+definition env_quotient :: "nat set \<Rightarrow> ('a env) quotient" ("\<bbbE>")
+  where "env_quotient I = (/\<equiv>I /\<Rightarrow> \<U>)"
+
+lemma env_subset: "A \<subseteq> B \<Longrightarrow> \<bbbE> B /\<le> \<bbbE> A"
+  by (simp add: env_quotient_def fun_quotient_subset_weak_intro set_quotient_subset_weak)
+  
+lemma env_subset_mod: "A \<subseteq> B \<Longrightarrow> env1 = env2 (mod \<bbbE> B) \<Longrightarrow> env1 = env2 (mod \<bbbE> A)"
+  by (meson env_subset qsubset_mod_weak)
+
+lemma env_app: "i \<in> I \<Longrightarrow> env1 = env2 (mod \<bbbE> I) \<Longrightarrow> env1 i = env2 i (mod \<U>)"
+  by (simp add: env_quotient_def fun_quotient_app_mod set_quotient_mod)
+
+lemma env_mod: "(env1 = env2 (mod \<bbbE> I)) = (\<forall> i \<in> I. env1 i = env2 i (mod \<U>))"
+  by (smt (verit, best) env_quotient_def fun_quotient_mod qequal_fun_def set_quotient_mod)
+
+subsection \<open>Evaluation\<close>
+
+fun beval :: "bterm \<Rightarrow> 'a valuation \<Rightarrow> 'a env \<Rightarrow> 'a" ("\<langle>_; _, _\<rangle>") where
+  "beval (FreeVar x ts) \<upsilon> env = \<upsilon> (x, length ts) (\<section>map t = ts!_. beval t \<upsilon> env)"
+| "beval (BoundVar i) \<upsilon> env = env i" 
+| "beval (Abstr a ts) \<upsilon> env = (\<O>!!a) (\<section>map t = ts!i. 
+     (\<lambda> us. beval t \<upsilon> (env \<up> \<section>v a {a!\<natural>i := us})))" 
+
+lemma beval_modulo:
+  "bwf t \<Longrightarrow>
+   bfrees t \<subseteq> X \<Longrightarrow> 
+   \<tau> = \<upsilon> (mod \<bbbV> X) \<Longrightarrow> 
+   unbounds t \<subseteq> I \<Longrightarrow>
+   env1 = env2 (mod \<bbbE> I) \<Longrightarrow>
+   beval t \<tau> env1 = beval t \<upsilon> env2 (mod \<U>)"
+proof (induct t arbitrary: env1 env2 I)
+  case (FreeVar x ts)
+  have "(x, length ts) \<in> bfrees (FreeVar x ts)"
+    by (simp add: union_indexed_fold)
+  then have x: "(x, length ts) \<in> X"
+    using FreeVar.prems(2) by blast
+  have bfrees: "\<And> i. i < length ts \<Longrightarrow> bfrees (ts ! i) \<subseteq> X" using bfrees_freeVar_arg
+    using FreeVar.prems(2) by blast
+  show ?case apply simp 
+    apply (rule valuation_quotient_app[where X="X"])
+    using FreeVar apply simp
+    apply (simp add: x)
+    apply (auto simp add: vector_quotient_mod qequal_vector_def)
+    apply (rule FreeVar(1))
+    apply simp
+    apply (erule bwf_freeVar_arg[OF FreeVar.prems(1)])
+    apply (erule bfrees)
+    using FreeVar apply simp
+    apply force
+    apply (rule env_subset_mod[where B = "I"])
+    apply (meson FreeVar.prems(4) sigloc.unbounds_freeVar_arg subset_trans)
+    using FreeVar apply simp
+    done
+next
+  case (BoundVar i)
+  have i: "i \<in> I"
+    using BoundVar.prems(4) by auto
+  show ?case 
+    apply simp 
+    using BoundVar i env_app 
+    by force
+next
+  case (Abstr a ts)
+  have valid: "\<checkmark> a"
+    using Abstr.prems(1) by force
+  have length_ts: "\<section>a a = length ts"
+    using Abstr.prems(1) by force
+  show ?case 
+    apply simp
+    apply (rule operator_appeq_intro[of "\<O> !! a" \<U> "\<S> !! a"])
+    using valid valid_in_operators apply force
+    apply (simp add: length_ts)+
+    apply (auto simp add: operations_mod)
+    apply (rule Abstr(1))
+    apply simp
+    using Abstr.prems(1) sigloc.bwf_abstr_arg apply blast
+    using Abstr.prems(2) bfrees_abstr_arg apply blast
+    using Abstr.prems(3) apply blast
+    apply (rule unbounds_bwf_abstr[where a=a], simp)
+    using Abstr apply simp
+    apply (auto simp add: env_mod union_unindexed_fold)
+    apply (subst env_app_noupdate[where env=env1])
+    using length_ts finite_shape_deps valid apply presburger
+    apply (metis (no_types, lifting) erase_bottom_indices length_ts linorder_not_le shape_deps_valence) 
+    apply (subst env_app_noupdate[where env=env2])
+    using length_ts finite_shape_deps valid apply presburger
+    apply (metis (no_types, lifting) erase_bottom_indices length_ts linorder_not_le shape_deps_valence) 
+    apply (simp add: env_raised_app)
+    apply (rule env_app[where I="I"])
+    using upper_bound_unbounds_abstr_arg erase_bottom_indices
+    apply (metis (no_types, lifting) Abstr.prems(4) subset_eq undo_raise_indices 
+           upper_bound_erased_unbounds_abstr_arg)
+    using Abstr apply simp
+    apply (subst env_app_update[where env=env1])
+    using finite_shape_deps length_ts valid apply presburger
+    apply simp
+    apply (subst env_app_update[where env=env2])
+    using finite_shape_deps length_ts valid apply presburger
+    apply simp
+    apply (rule  vector_quotient_nth_mod)
+    apply auto using valid
+    using length_ts sigloc.finite_shape_deps upper_bound_index_sorted_list by presburger
+qed
 
 end
 
